src/ocamlmm/OCamlToimm_s_prog_pair_step.v
@@ -1,0 +1,490 @@
+(******************************************************************************)
+(** * ocaml MM is weaker than IMM_S   *)
+(******************************************************************************)
+Require Import Classical Peano_dec.
+From hahn Require Import Hahn.
+Require Import Omega.
+Require Import Events.
+Require Import Execution.
+Require Import Execution_eco.
+Require Import imm_common.
+Require Import imm_s_hb.
+Require Import imm_s.
+Require Import OCaml.
+Require Import OCamlToimm_s.
+Require Import OCamlToimm_s_prog. 
+Require Import OCamlToimm_s_prog_compilation. 
+Require Import OCamlToimm_s_prog_bounded_properties. 
+Require Import Utils.
+Require Import ClosuresProperties. 
+Require Import Prog.
+Require Import ProgToExecution.
+Require Import ProgToExecutionProperties.
+Require Import Logic.Decidable. 
+From PromisingLib Require Import Basic Loc.
+Require Import Basics. 
+Set Implicit Arguments.
+
+Section PairStep.
+  Notation "'E' G" := G.(acts_set) (at level 1).
+  Notation "'R' G" := (fun a => is_true (is_r G.(lab) a)) (at level 1).
+  Notation "'W' G" := (fun a => is_true (is_w G.(lab) a)) (at level 1).
+  Notation "'RW' G" := (R G ∪₁ W G) (at level 1).
+  (* Warning: F implicitly means at least acq/rel fence *)
+  Notation "'F' G" := (fun a => is_true (is_nonnop_f G.(lab) a)) (at level 1).
+  Notation "'ORlx' G" := (fun a => is_true (is_only_rlx G.(lab) a)) (at level 1).
+  Notation "'Sc' G" := (fun a => is_true (is_sc G.(lab) a)) (at level 1). 
+  Notation "'Acq' G" := (fun a => is_true (is_acq G.(lab) a)) (at level 1). 
+  Notation "'Acqrel' G" := (fun a => is_true (is_acqrel G.(lab) a)) (at level 1). 
+  Notation "'R_ex' G" := (fun a => is_true (R_ex G.(lab) a)) (at level 1).
+  Notation "'hbo'" := (OCaml.hb). 
+  Notation "'same_loc' G" := (same_loc G.(lab)) (at level 1).
+  Notation "'Tid_' t" := (fun x => tid x = t) (at level 1).
+
+  Lemma blockstep_implies_steps bst1 bst2 tid
+        (BLOCK_STEPS: (block_step tid)＊ bst1 bst2): 
+    (step tid)＊ (bst2st bst1) (bst2st bst2). 
+  Proof.
+    apply crt_num_steps. apply crt_num_steps in BLOCK_STEPS. desc.
+    generalize dependent bst1. generalize dependent bst2. induction n.
+    { ins. red in BLOCK_STEPS. desc.
+      exists 0. apply steps0. congruence. }
+    ins. red in BLOCK_STEPS. destruct BLOCK_STEPS as [bst' [BLOCK_STEPS1 BLOCK_STEPS2]].
+    specialize (IHn _ _ BLOCK_STEPS1). destruct IHn as [n' STEPS1].
+    red in BLOCK_STEPS2. desc. red in BLOCK_STEPS2. desc. 
+    exists (n' + length block).
+    forward eapply (steps_split (step tid) n' (length block) _ (bst2st bst1) (bst2st bst2)) as SPLIT; auto. 
+    apply SPLIT. exists (bst2st bst'). split; auto.
+    Unshelve. auto.
+  Qed. 
+
+  Lemma flatten_split {A: Type} (ll: list (list A)) bi (INDEX: bi < length ll):
+    flatten ll = flatten (firstn bi ll) ++ flatten (skipn bi ll).
+  Proof. ins. rewrite <- flatten_app. rewrite firstn_skipn. auto. Qed. 
+    
+  Lemma pair_step sto bsti (MM_SIM: mm_similar_states sto bsti)
+        tid bsti' (OSEQ_STEP: omm_block_step tid bsti bsti')
+        (BLOCK_REACH: (block_step tid)＊ (binit (binstrs bsti)) bsti):
+    exists sto', Ostep tid sto sto' /\ mm_similar_states sto' bsti'.
+  Proof.
+    pose proof (block_step_nonterminal (bs_extract OSEQ_STEP)) as BST_NONTERM. 
+    pose proof (BPC_CHANGE OSEQ_STEP) as BPC'. 
+    red in OSEQ_STEP. destruct OSEQ_STEP as [block [BLOCK_STEP_ COMP_BLOCK]].
+    forward eapply (@SAME_BINSTRS bsti bsti' tid) as BINSTRS_SAME.
+    { red. eauto. }
+    desc.
+    red in BLOCK_STEP_. desc.
+    inversion COMP_BLOCK.
+    all: rename H into OINSTR.
+    all: rename H0 into BLOCK_CONTENTS.
+    all: subst; simpl in *.
+    - remember (bst2st bsti) as sti. remember (bst2st bsti') as sti'. 
+      apply (same_relation_exp (seq_id_l (step tid))) in BLOCK_STEP.
+      assert (AT_PC: Some ld = nth_error (instrs sti) (pc sti)).
+      { replace (instrs sti) with (flatten (binstrs bsti)).
+        2: { unfold bst2st in Heqsti. subst. auto. }
+        replace (pc sti) with (length (flatten (firstn (bpc bsti) (binstrs bsti)))).
+        2: { unfold bst2st in Heqsti. subst. auto. }
+        rewrite <- (firstn_skipn (bpc bsti) (binstrs bsti)) in AT_BLOCK. 
+        rewrite nth_error_app2 in AT_BLOCK.
+        2: { apply firstn_le_length. }
+        rewrite firstn_length_le in AT_BLOCK; [| omega]. 
+        rewrite Nat.sub_diag in AT_BLOCK.
+        rewrite (@flatten_split _ (binstrs bsti) (bpc bsti)); [| auto]. 
+        rewrite nth_error_app2; [| omega].
+        rewrite Nat.sub_diag.        
+        assert (forall {A: Type} l (x: A), Some x = nth_error l 0 -> exists l', l = x :: l'). 
+        { ins. destruct l; vauto. }
+        apply H in AT_BLOCK. desc.
+        rewrite AT_BLOCK. simpl. auto. }
+      red in BLOCK_STEP. desc. red in BLOCK_STEP. desc.
+      rewrite <- AT_PC in ISTEP. inversion ISTEP as [EQ]. clear ISTEP. 
+      inversion ISTEP0.
+      all: rewrite II in EQ.
+      all: try discriminate.
+      rewrite EQ in *. subst instr. 
+      set (sto' :=
+             {| instrs := instrs sto;
+                pc := pc sto + 1;
+                G := add (G sto) tid (eindex sto)
+                         (Aload false ord (RegFile.eval_lexpr (regf sti) lexpr) val) ∅
+                         (DepsFile.lexpr_deps (depf sti) lexpr) (ectrl sti) ∅;
+                         eindex := eindex sto + 1;
+                regf := RegFun.add reg val (regf sto);
+                depf := RegFun.add reg (eq (ThreadEvent tid (eindex sti))) (depf sto);
+                ectrl := ectrl sto |}).
+      red in MM_SIM. desc.
+      assert (REGF_EQ: regf sto = regf sti). 
+      { rewrite MM_SIM2. vauto. }
+      assert (DEPF_EQ: depf sto = depf sti). 
+      { rewrite MM_SIM3. vauto. }
+      assert (EINDEX_EQ: eindex sto = eindex sti). 
+      { rewrite MM_SIM5. vauto. }
+      assert (ECTRL_EQ: ectrl sto = ectrl sti). 
+      { rewrite MM_SIM4. vauto. }
+      exists sto'. splits.
+      { red. exists lbls. red. splits; [subst; simpl; auto| ].
+        exists ld. exists 0. splits.
+        { assert (exists oinstr, Some oinstr = nth_error (instrs sto) (pc sto)).
+          { apply OPT_VAL. apply nth_error_Some.
+            rewrite MM_SIM0.
+            replace (length (instrs sto)) with (length (binstrs bsti)); auto. 
+            symmetry. apply compilation_same_length. auto. }
+          desc. pose proof (every_instruction_compiled MM_SIM (pc sto)).
+          forward eapply H0 as COMP; eauto.
+          { replace (pc sto) with (bpc bsti). eauto. }
+          cut (ld = oinstr); [congruence| ].
+          inversion COMP. vauto. }
+        pose proof (@Oload tid lbls sto sto' ld 0 Orlx reg lexpr val l) as OMM_STEP.
+        assert (ORD_RLX: ord = Orlx). 
+        { subst ld. congruence. }
+        rewrite ORD_RLX, REGF_EQ, DEPF_EQ, EINDEX_EQ, ECTRL_EQ in *. 
+        forward eapply OMM_STEP; eauto.
+        { subst sto'. simpl. rewrite ORD_RLX, EINDEX_EQ, Nat.add_0_r. auto. }
+        { subst sto'. simpl. rewrite EINDEX_EQ, Nat.add_0_r.  auto. }
+        { subst sto'. simpl. rewrite REGF_EQ. auto. }
+        subst sto'. simpl. rewrite DEPF_EQ. auto. }
+      (* assert (LAB_EQ: lab (G sto) = lab (G sti)). *)
+      (* { red in MM_SIM1. desc. vauto. } *)
+      red. splits.
+      { subst sto'. simpl. rewrite <- BINSTRS_SAME. auto. }
+      {  subst sto'. simpl. destruct BPC' as [BPC' | BPC']. 
+         - rewrite BPC'. rewrite MM_SIM0. auto.
+         - desc. congruence. }
+      { red.
+        assert (exists n_steps, (step tid) ^^ n_steps (init (instrs sti)) sti) as [n_steps REACH].
+        { apply crt_num_steps. 
+          subst sti.
+          replace (init (instrs (bst2st bsti))) with (bst2st (binit (binstrs bsti))). 
+          { apply blockstep_implies_steps. auto. }
+          unfold bst2st, init. simpl. auto. }
+        splits.
+        { replace (bG bsti') with (G sti') by vauto.
+          rewrite (@E_ADD).
+          2: { repeat eexists. } 
+          rewrite (@E_ADD (G sti) (G sti')).
+          2: { repeat eexists. eapply UG. }
+
+          desc. 
+          forward eapply (@label_set_step (@is_r actid) r_matcher sti sti' tid) as R_EXT; eauto. 
+          { apply r_pl. }
+          { forward eapply nonnop_bounded; eauto.
+            { generalize r_pl. eauto. }
+            vauto. } 
+          forward eapply (@label_set_step (@is_w actid) w_matcher sti sti' tid) as W_EXT; eauto. 
+          { apply w_pl. }
+          { forward eapply nonnop_bounded; eauto.
+            { generalize w_pl. eauto. }
+            vauto. } 
+          rewrite R_EXT, W_EXT. simpl in *.
+          arewrite (rmw (G sti') ≡ rmw (G sti)).
+          { rewrite UG. vauto. }
+          rewrite EINDEX_EQ, set_union_empty_r. 
+          remember (eq (ThreadEvent tid (eindex sti))) as nev.
+          rewrite set_unionA, (set_unionC _ (W (G sti))), <- set_unionA.
+          rewrite set_inter_union_l. apply set_equiv_union.
+          { rewrite set_inter_minus_r.
+            arewrite (E (G sti) ∩₁ (RW (G sti) ∪₁ nev) ≡₁ E (G sti) ∩₁ RW (G sti)).
+            { rewrite set_inter_union_r. 
+              arewrite (E (G sti) ∩₁ nev ≡₁ ∅); [| basic_solver ].
+              split; [| basic_solver].
+              rewrite E_bounded; eauto. vauto.
+              red. ins. red in H. desc. rewrite <- H0 in H. simpl in H. omega. }
+            red in MM_SIM1. desc.
+            replace (G sti) with (bG bsti) by vauto.
+            rewrite <- set_inter_minus_r. auto. }
+          split; [| basic_solver].
+          apply set_subset_inter_r. split; [basic_solver| ].
+          apply inclusion_minus. split; [basic_solver| ]. 
+          subst nev. red. ins. red in H. desc. red. 
+          forward eapply rmw_bibounded; eauto.
+          ins. red in H1. desc.
+          red in H0. desc. specialize (H1 x y).
+          pose proof (H1 H0). desc. 
+          rewrite <- H in H2. simpl in H2. omega. }
+        (* **** *)
+        replace (bG bsti') with (G sti'); [| vauto ]. 
+        subst sto'. rewrite UG. simpl.
+        ins. unfold add, acts_set in EGOx. simpl in EGOx.
+        red in MM_SIM. rewrite <- EINDEX_EQ. destruct EGOx.
+        + rewrite H. do 2 rewrite upds. auto.
+        + assert (x <> ThreadEvent tid (eindex sto)) as NEQ.
+          { red. ins. rewrite H0 in H.
+            forward eapply E_bounded as BOUND; eauto.
+            rewrite  EINDEX_EQ in H0, H.
+            assert (E (G sti) x) as EGIx.
+            { red in MM_SIM1. desc. red in RESTR_EVENTS. desc.
+              red in RESTR_EVENTS. forward eapply (RESTR_EVENTS x); vauto.
+              basic_solver. }
+            red in BOUND. specialize (BOUND x EGIx).
+            rewrite H0 in BOUND. simpl in BOUND. omega. }
+          rewrite updo; auto. rewrite updo; auto. 
+          red in MM_SIM1. desc. replace (G sti) with (bG bsti); [| vauto ]. 
+          apply SAME_LAB. auto. }
+      { subst sto'. replace (bregf bsti') with (regf sti'); [| vauto ].
+        simpl. congruence. }
+      { subst sto'. replace (bdepf bsti') with (depf sti'); [| vauto ].
+        simpl. congruence. }
+      { subst sto'. replace (bectrl bsti') with (ectrl sti'); [| vauto ].
+        simpl. congruence. }
+      { subst sto'. replace (beindex bsti') with (eindex sti'); [| vauto ].
+        simpl. congruence. }
+    - remember (bst2st bsti) as sti. remember (bst2st bsti') as sti'.
+      apply (same_relation_exp (seqA _ _ _)) in BLOCK_STEP. 
+      rewrite (same_relation_exp (seq_id_l _)) in BLOCK_STEP.
+      rename sti' into sti''. rename bsti' into bsti''.
+      red in BLOCK_STEP. destruct BLOCK_STEP as [sti' [STEP' STEP'']]. 
+      assert (AT_PC: Some f = nth_error (instrs sti) (pc sti)).
+      { replace (instrs sti) with (flatten (binstrs bsti)).
+        2: { unfold bst2st in Heqsti. subst. auto. }
+        replace (pc sti) with (length (flatten (firstn (bpc bsti) (binstrs bsti)))).
+        2: { unfold bst2st in Heqsti. subst. auto. }
+        rewrite <- (firstn_skipn (bpc bsti) (binstrs bsti)) in AT_BLOCK. 
+        rewrite nth_error_app2 in AT_BLOCK.
+        2: { apply firstn_le_length. }
+        rewrite firstn_length_le in AT_BLOCK; [| omega]. 
+        rewrite Nat.sub_diag in AT_BLOCK.
+        rewrite (@flatten_split _ (binstrs bsti) (bpc bsti)); [| auto]. 
+        rewrite nth_error_app2; [| omega].
+        rewrite Nat.sub_diag.        
+        assert (forall {A: Type} l (x: A), Some x = nth_error l 0 -> exists l', l = x :: l'). 
+        { ins. destruct l; vauto. }
+        apply H in AT_BLOCK. desc.
+        rewrite AT_BLOCK. simpl. auto. }
+      assert (AT_PC': Some st = nth_error (instrs sti) (pc sti + 1)).
+      { replace (instrs sti) with (flatten (binstrs bsti)).
+        2: { unfold bst2st in Heqsti. subst. auto. }
+        replace (pc sti) with (length (flatten (firstn (bpc bsti) (binstrs bsti)))).
+        2: { unfold bst2st in Heqsti. subst. auto. }
+        rewrite <- (firstn_skipn (bpc bsti) (binstrs bsti)) in AT_BLOCK. 
+        rewrite nth_error_app2 in AT_BLOCK.
+        2: { apply firstn_le_length. }
+        rewrite firstn_length_le in AT_BLOCK; [| omega]. 
+        rewrite Nat.sub_diag in AT_BLOCK.
+        rewrite (@flatten_split _ (binstrs bsti) (bpc bsti)); [| auto]. 
+        rewrite nth_error_app2; [| omega].
+        rewrite minus_plus. 
+        assert (forall {A: Type} l (x: A), Some x = nth_error l 0 -> exists l', l = x :: l'). 
+        { ins. destruct l; vauto. }
+        apply H in AT_BLOCK. desc.
+        rewrite AT_BLOCK. simpl. auto. }      
+
+      red in STEP'. desc. red in STEP'. desc.
+      rewrite <- AT_PC in ISTEP. inversion ISTEP as [EQ]. clear ISTEP. 
+      inversion ISTEP0.
+      all: rewrite II in EQ.
+      all: try discriminate.
+      rewrite EQ in *. subst instr. 
+      set (sto' :=
+             {| instrs := instrs sto;
+                pc := pc sto;
+                G := G sto;
+                eindex := eindex sto;
+                regf := regf sto;
+                depf := depf sto;
+                ectrl := ectrl sto |}).
+
+      red in STEP''. desc. red in STEP''. desc.
+      rewrite <- INSTRS, UPC, <- AT_PC' in ISTEP. inversion ISTEP as [EQ']. clear ISTEP. 
+      inversion ISTEP1.
+      all: rewrite II in EQ'.
+      all: try discriminate.
+      rewrite EQ' in *. subst instr.
+      rename x into xmd. 
+      set (sto'' :=
+             {| instrs := instrs sto;
+                pc := pc sto' + 1;
+                (* G := add (G sto') tid (eindex sto') (Astore x ord0 l v) *)
+                G := add (G sto') tid (eindex sto' + 1) (Astore xmd ord0 l v)
+                         (DepsFile.expr_deps (depf sto') expr)
+                         (DepsFile.lexpr_deps (depf sto') lexpr) (ectrl sto') ∅;
+                eindex := eindex sto' + 2;
+                regf := regf sto';
+                depf := depf sto';
+                ectrl := ectrl sto' |}).
+
+      red in MM_SIM. desc.
+      assert (REGF_EQ: regf sto = regf sti). 
+      { rewrite MM_SIM2. vauto. }
+      assert (DEPF_EQ: depf sto = depf sti). 
+      { rewrite MM_SIM3. vauto. }
+      assert (EINDEX_EQ: eindex sto = eindex sti). 
+      { rewrite MM_SIM5. vauto. }
+      assert (ECTRL_EQ: ectrl sto = ectrl sti). 
+      { rewrite MM_SIM4. vauto. }
+      
+      exists sto''. splits.
+      { red. exists lbls0. red. splits; [subst; simpl; auto| ].
+        exists st. exists 1. splits.
+        { assert (exists oinstr, Some oinstr = nth_error (instrs sto) (pc sto)).
+          { apply OPT_VAL. apply nth_error_Some.
+            rewrite MM_SIM0.
+            replace (length (instrs sto)) with (length (binstrs bsti)); auto. 
+            symmetry. apply compilation_same_length. auto. }
+          desc. pose proof (every_instruction_compiled MM_SIM (pc sto)).
+          forward eapply H0 as COMP; eauto.
+          { replace (pc sto) with (bpc bsti). eauto. }
+          cut (st = oinstr); [congruence| ].
+          inversion COMP. vauto. }
+        assert (ORD_RLX: ord0 = Orlx). 
+        { subst st. congruence. }
+        rewrite ORD_RLX in *. 
+        assert (Instr.store Orlx lexpr expr = Instr.store Orlx loc val) by vauto.
+        inversion H. subst lexpr. subst expr. clear H. 
+
+        
+        (* pose proof (@Ostore tid lbls0 sto sto'' st 2 (gt_Sn_O 1) Orlx loc val l v) as OMM_STEP. *)
+        pose proof (@Ostore tid lbls0 sto sto'' st 1 Orlx loc val l v) as OMM_STEP.
+
+        
+        (* TODO: ???*)
+        (* rewrite ORD_RLX, REGF_EQ, DEPF_EQ, EINDEX_EQ, ECTRL_EQ in *. *)
+        (*********)
+        forward eapply OMM_STEP; eauto.
+        (* TODO: modify equalities above to operate with sti' ? *)
+        { rewrite REGF_EQ, <- UREGS. auto. }
+        { rewrite REGF_EQ, <- UREGS. auto. }
+        { subst sto''. subst sto'. simpl. rewrite ORD_RLX, EINDEX_EQ.
+          unfold add at 1. simpl. basic_solver.  }
+        subst sto''. subst sto'. simpl. omega. }
+      red. splits.
+      { subst sto''. simpl. rewrite <- BINSTRS_SAME. auto. }
+      { subst sto''. simpl. destruct BPC' as [BPC' | BPC']. 
+         - rewrite BPC'. rewrite MM_SIM0. auto.
+         - desc. congruence. }
+      { red.
+        assert (exists n_steps, (step tid) ^^ n_steps (init (instrs sti)) sti) as [n_steps REACH].
+        { apply crt_num_steps. 
+          subst sti.
+          replace (init (instrs (bst2st bsti))) with (bst2st (binit (binstrs bsti))). 
+          { apply blockstep_implies_steps. auto. }
+          unfold bst2st, init. simpl. auto. }
+          assert (exists n_steps', (step tid) ^^ n_steps' (init (instrs sti')) sti') as [n_steps' REACH'].
+          { exists (n_steps + 1). rewrite Nat.add_1_r. apply step_prev.
+            exists sti. split.
+            { rewrite <- INSTRS. auto. }
+            red. exists lbls. red. splits; auto.
+            eexists. eauto. }        
+        splits.
+        { replace (bG bsti'') with (G sti'') by vauto.
+          rewrite (@E_ADD).
+          2: { repeat eexists. } 
+          rewrite (@E_ADD (G sti') (G sti'') tid (eindex sti + 1)).
+          2: { repeat eexists. rewrite <- UINDEX. eapply UG0. }
+          rewrite (@E_ADD (G sti) (G sti') tid (eindex sti)).
+          2: { repeat eexists. eapply UG. }
+          
+          desc. 
+          forward eapply (@label_set_step (@is_r actid) r_matcher sti sti' tid) as R_EXT; eauto. 
+          { apply r_pl. }
+          { forward eapply (@nonnop_bounded n_steps); eauto.
+            { generalize r_pl. eauto. }
+            vauto. } 
+          forward eapply (@label_set_step (@is_w actid) w_matcher sti sti' tid) as W_EXT; eauto. 
+          { apply w_pl. }
+          { forward eapply (@nonnop_bounded n_steps); eauto.
+            { generalize w_pl. eauto. }
+            vauto. } 
+          
+          desc. 
+          forward eapply (@label_set_step (@is_r actid) r_matcher sti' sti'' tid) as R_EXT'; eauto. 
+          { apply r_pl. }
+          { forward eapply (@nonnop_bounded n_steps'); eauto.
+            { generalize r_pl. eauto. }
+            vauto. } 
+          forward eapply (@label_set_step (@is_w actid) w_matcher sti' sti'' tid) as W_EXT'; eauto. 
+          { apply w_pl. }
+          { forward eapply (@nonnop_bounded n_steps'); eauto.
+            { generalize w_pl. eauto. }
+            vauto. } 
+
+          rewrite W_EXT', R_EXT', R_EXT, W_EXT. simpl in *.
+          arewrite (rmw (G sti'') ≡ rmw (G sti)).
+          { rewrite UG0, UG. vauto. }
+          rewrite EINDEX_EQ, !set_union_empty_r. 
+          remember (eq (ThreadEvent tid (eindex sti))) as nev.
+          rewrite UINDEX. remember (eq (ThreadEvent tid (eindex sti + 1))) as nev'.
+          rewrite <- set_unionA, set_unionA. 
+          rewrite set_inter_union_l. apply set_equiv_union.
+          { rewrite set_inter_minus_r.
+            arewrite (E (G sti) ∩₁ (RW (G sti) ∪₁ nev') ≡₁ E (G sti) ∩₁ RW (G sti)).
+            { rewrite set_inter_union_r. 
+              arewrite (E (G sti) ∩₁ nev' ≡₁ ∅); [| basic_solver ].
+              split; [| basic_solver].
+              rewrite E_bounded; eauto. vauto.
+              red. ins. red in H. desc. rewrite <- H0 in H. simpl in H. omega. }
+            red in MM_SIM1. desc.
+            replace (G sti) with (bG bsti) by vauto.
+            rewrite <- set_inter_minus_r. auto. }
+          split.
+          2: { rewrite set_inter_union_l. apply set_subset_union_l.
+               split; [| basic_solver].
+               rewrite set_inter_minus_r. rewrite set_inter_union_r.
+               arewrite (nev ∩₁ nev' ≡₁ ∅).
+               { subst. red. split; [| basic_solver].
+                 red. ins. red in H. desc. rewrite <- H in H0.
+                 inversion H0. omega. }
+               arewrite (nev ∩₁ RW (G sti) ≡₁ ∅).
+               2: basic_solver.
+               red. split; [| basic_solver]. 
+               red. ins. red in H. desc. rewrite Heqnev in H.
+               red in H0. destruct H0.
+               + forward eapply (@nonnop_bounded n_steps (@is_r actid) r_matcher sti tid) as R_BOUNDED; eauto. 
+               { apply r_pl. }
+               { red. vauto. }
+                 do 2 red in R_BOUNDED. specialize (R_BOUNDED x H0).
+                 rewrite <- H in R_BOUNDED. simpl in R_BOUNDED. omega.
+               + forward eapply (@nonnop_bounded n_steps (@is_w actid) w_matcher sti tid) as W_BOUNDED; eauto. 
+               { apply w_pl. }
+               { red. vauto. }
+                 do 2 red in W_BOUNDED. specialize (W_BOUNDED x H0).
+                 rewrite <- H in W_BOUNDED. simpl in W_BOUNDED. omega. }
+               
+          apply set_subset_inter_r. split; [basic_solver| ].
+          apply inclusion_minus. split; [basic_solver| ]. 
+          subst nev. red. ins. red in H. desc. red. 
+          forward eapply rmw_bibounded; eauto.
+          ins. red in H1. desc.
+          red in H0. desc. specialize (H1 x y).
+
+          assert (rmw (G sti') x y) as RMW'xy. 
+          { assert (rmw (G sti') ≡ rmw (G sti)). 
+            { rewrite UG. vauto. }
+            apply (same_relation_exp H2). auto. }
+          
+          pose proof (H1 RMW'xy). desc. 
+          rewrite Heqnev' in H. rewrite <- H in H2. simpl in H2. omega. }
+        replace (bG bsti'') with (G sti''); [| vauto ]. 
+        subst sto''. rewrite UG0, UG. simpl.
+        ins. unfold add, acts_set in EGOx. simpl in EGOx.
+        rewrite UINDEX, <- EINDEX_EQ.
+        destruct EGOx.
+        + rewrite H. do 2 rewrite upds. auto.
+        + assert (index x < eindex sto) as NEQ.
+          { destruct (Const.lt_decidable (index x) (eindex sto)); auto.
+            exfalso. 
+            forward eapply (@E_bounded n_steps tid sti) as BOUND; eauto.
+            assert (E (G sti) x) as EGIx.
+            { red in MM_SIM1. desc. red in RESTR_EVENTS. desc.
+              red in RESTR_EVENTS. forward eapply (RESTR_EVENTS x); vauto.
+              basic_solver. }
+            red in BOUND. specialize (BOUND x EGIx).
+            omega. }
+          rewrite updo. rewrite updo. rewrite updo.
+          2, 3, 4: red; ins; rewrite H0 in NEQ; simpl in NEQ; omega.
+          red in MM_SIM1. desc. replace (G sti) with (bG bsti); [| vauto ]. 
+          apply SAME_LAB. auto. }
+      { subst sto'. replace (bregf bsti'') with (regf sti''); [| vauto ].
+        simpl. congruence. }
+      { subst sto'. replace (bdepf bsti'') with (depf sti''); [| vauto ].
+        simpl. congruence. }
+      { subst sto'. replace (bectrl bsti'') with (ectrl sti''); [| vauto ].
+        simpl. congruence. }
+      { subst sto'. replace (beindex bsti'') with (eindex sti''); [| vauto ].
+        simpl. rewrite UINDEX0, UINDEX. omega. }
+      (* - .....*)
+      (* - .....*)
+      (* - .....*)
+  Admitted.
+
+End PairStep.  
