src/ocamlmm/Utils.v
@@ -1,0 +1,22 @@
+Require Import Classical Peano_dec.
+From hahn Require Import Hahn.
+Set Implicit Arguments.
+
+
+Lemma inclusion_minus {A: Type} (s u m: A -> Prop):
+  s ⊆₁ u \₁ m <-> s ⊆₁ u /\ s ∩₁ m ⊆₁ ∅.
+Proof.
+  (*link to similar lemma here*)
+Admitted. 
+
+Lemma OPT_VAL: forall {A: Type} (opt: option A), opt <> None <-> exists o, Some o = opt.
+Proof. 
+  intros. destruct opt eqn:v. 
+  - red. split; intros. 
+    + eexists. eauto.
+    + discriminate.
+  - red. split; intros.
+    + intuition.
+    + destruct H. discriminate H.  
+Qed.  
+
